<?xml version="1.0" encoding="utf-8" ?>

<!DOCTYPE rdf:RDF [
    <!ENTITY owl "http://www.w3.org/2002/07/owl#" >
    <!ENTITY xsd "http://www.w3.org/2001/XMLSchema#" >
    <!ENTITY rdfs "http://www.w3.org/2000/01/rdf-schema#" >
    <!ENTITY rdf "http://www.w3.org/1999/02/22-rdf-syntax-ns#" >
]>

<rdf:RDF 
   xmlns="http://docs.staite.net/uni-co7216-cwk2#"
   xml:base="http://docs.staite.net/uni-co7216-cwk2"
   xmlns:rdfs="http://www.w3.org/2000/01/rdf-schema#"
   xmlns:owl="http://www.w3.org/2002/07/owl#"
   xmlns:xsd="http://www.w3.org/2001/XMLSchema#"
   xmlns:rdf="http://www.w3.org/1999/02/22-rdf-syntax-ns#">
    
   <owl:Ontology rdf:about="http://docs.staite.net/uni-co7216-cwk2"></owl:Ontology>
   
   <!-- **************************************** -->   
   <!-- CLASSES AND PROPERTIES FROM COURSEWORK 1 -->  
   <!-- **************************************** -->
   
   <!-- 
      
      Note that we havn't included rdfs:comment for each
      of the classes and properties taken directly from 
      the first coursework. If you need the comments for 
      those please refer to our coursework 1 submission.      
      
   -->
   
   <owl:Class rdf:about="#Region"></owl:Class>   
   <owl:Class rdf:about="#News"></owl:Class>
   <owl:Class rdf:about="#NewsSubject"></owl:Class>   
   <owl:Class rdf:about="#NewsSource"></owl:Class>
   <owl:Class rdf:about="#Person"></owl:Class>

   <owl:Class rdf:about="#Journalist">
      <rdfs:subClassOf rdf:resource="#Person" />
   </owl:Class>

   <owl:Class rdf:about="#Technology">
      <rdfs:subClassOf rdf:resource="#NewsSubject" />
   </owl:Class>

   <owl:Class rdf:about="#Software">
      <rdfs:subClassOf rdf:resource="#Technology" />
   </owl:Class>

   <owl:Class rdf:about="#App">
      <rdfs:subClassOf rdf:resource="#Software" />
   </owl:Class>

   <owl:Class rdf:about="#OpenSource">
      <rdfs:subClassOf rdf:resource="#Technology" />
   </owl:Class>

   <owl:Class rdf:about="#Device">
      <rdfs:subClassOf rdf:resource="#Technology" />
   </owl:Class>

   <owl:Class rdf:about="#Mobile">
      <rdfs:subClassOf rdf:resource="#Device" />
   </owl:Class>

   <owl:Class rdf:about="#Company">
        <rdfs:subClassOf rdf:resource="#NewsSubject" />
    </owl:Class>

   <owl:Class rdf:about="#Newspaper">
      <rdfs:subClassOf rdf:resource="#NewsSource" />
   </owl:Class>
   
   <owl:ObjectProperty rdf:about="#worksForSource">
      <rdfs:domain rdf:resource="#Journalist" />
      <rdfs:range rdf:resource="#NewsSource" />
   </owl:ObjectProperty>

   <owl:ObjectProperty rdf:about="#worksForSource">
      <rdfs:domain rdf:resource="#Journalist" />
      <rdfs:range rdf:resource="#NewsSource" />
   </owl:ObjectProperty>

    <owl:ObjectProperty rdf:about="#runsSoftware">
        <rdfs:domain rdf:resource="#Device" />
        <rdfs:range rdf:resource="#Software" />
    </owl:ObjectProperty>

    <owl:ObjectProperty rdf:about="#builds">
        <rdfs:domain rdf:resource="#Company" />
        <rdfs:range rdf:resource="#Device" />
    </owl:ObjectProperty>

   <owl:ObjectProperty rdf:about="#hasCoverage">
      <rdfs:domain rdf:resource="#Newspaper" />
      <rdfs:range rdf:resource="#Region" />
   </owl:ObjectProperty>    

   <owl:ObjectProperty rdf:about="#hasCorrespondingWebsite">
      <rdfs:range rdf:resource="#NewsWebsite"/>
      <rdfs:domain rdf:resource="#Newspaper"/>
   </owl:ObjectProperty>

   <owl:ObjectProperty rdf:about="#runsSoftware">
      <rdfs:domain rdf:resource="#Device"/>
      <rdfs:range rdf:resource="#Software"/>
   </owl:ObjectProperty>

   <!-- **************************************** -->
   <!-- NEW CLASSES / PROPERTIES / RESTRICTIONS  -->
   <!-- **************************************** -->
   
   <owl:Class rdf:about="#Blogger">
   
      <rdfs:subClassOf rdf:resource="#Journalist" />
      <rdfs:subClassOf>
         <owl:Restriction>
            <owl:onProperty rdf:resource="#worksForSource" />
            <owl:someValuesFrom rdf:resource="#Blog" />
         </owl:Restriction>
      </rdfs:subClassOf>
      
      <rdfs:comment rdf:datatype="xsd:string">
      
         * This is a subclass restriction.
         * This is an existential restriction. 
         * This is an implicit cardinality restriction (min 1). 
         
         The class of people who are journalists and 
         work for at least 1 blog.         
      
      </rdfs:comment>
      
   </owl:Class>

   <!-- ========================================= -->

   <owl:ObjectProperty rdf:about="#runsOnDevice">

      <rdfs:domain rdf:resource="#Software" />
      <rdfs:range rdf:resource="#Device" />
      <owl:inverseOf rdf:resource="#runsSoftware" />

      <rdfs:comment rdf:datatype="xsd:string">
      
         * This is an object property.
         * This is an inverse property.
         * This is a (boring) domain restriction.
         * This is a (boring) range restriction.  
         
         A piece of software can run on 0 or more devices. 
      
      </rdfs:comment>

   </owl:ObjectProperty>

   <!-- ========================================= -->

   <owl:ObjectProperty rdf:about="#builtByCompany">

      <rdfs:domain rdf:resource="#Device" />
      <rdfs:range rdf:resource="#Company" />
      <owl:inverseOf rdf:resource="#builds" />

      <rdfs:comment rdf:datatype="xsd:string">
      
         * This is an object property.
         * This is an inverse property.
         * This is a (boring) domain restriction.
         * This is a (boring) range restriction.  
         
        A device is built by a company.
      
      </rdfs:comment>

   </owl:ObjectProperty>

   <!-- ========================================= -->

   <owl:Class rdf:about="#iPhoneDevice">
      
      <rdfs:subClassOf rdf:resource="#Mobile" />
      <rdfs:subClassOf>
         <owl:Restriction>
            <owl:onProperty rdf:resource="#builtByCompany" />
            <owl:hasValue rdf:resource="#Apple" />
         </owl:Restriction>
      </rdfs:subClassOf>

      <rdfs:comment>

         * This is a subclass restriction.
         * This is an (implicit) cardinality restriction (exactly 1).

         All mobile phones made by apple are iPhones. Note that
         the individuals are specific models like iPhone4S and
         iPhoneDevice is the class of these iPhone models. 

      </rdfs:comment>

   </owl:Class> 

   <!-- ========================================= -->

   <owl:Class rdf:about="#iPhoneApp">

      <rdfs:subClassOf rdf:resource="#App" />
      <rdfs:subClassOf>            
         <owl:Restriction>
            <owl:onProperty rdf:resource="#runsOnDevice" />
            <owl:allValuesFrom rdf:resource="#iPhoneDevice" />
         </owl:Restriction>
      </rdfs:subClassOf>

      <rdfs:comment rdf:datatype="xsd:string">

         * This is a subclass restriction.
         * This is a universal restriction. 

         The class of software that is open source. 

      </rdfs:comment>

   </owl:Class>
      
   <!-- ========================================= -->

   <owl:Class rdf:about="#OpenSourceSoftware">

      <rdfs:subClassOf rdf:resource="#Software" />
      <rdfs:subClassOf rdf:resource="#OpenSource" />

      <rdfs:comment rdf:datatype="xsd:string">

         * This is a subclass restriction.

         The class of software that is open source. 

      </rdfs:comment>

   </owl:Class>

   <!-- ========================================= -->

   <owl:DatatypeProperty rdf:about="#hasVersion">

      <rdfs:domain rdf:resource="#Software" />
      <rdfs:domain rdf:resource="#Device" />
      <rdfs:range rdf:resource="&xsd;string" />

      <rdfs:comment rdf:datatype="xsd:string">

         * This is a datatype property.
         * This is a (boring) domain restriction.
         * This is a (boring) range restriction.  

         A piece of software has a version. 
         A device has a version. 

      </rdfs:comment>

   </owl:DatatypeProperty>

   <!-- ========================================= -->

   <owl:DatatypeProperty rdf:about="#hasGBDiskCapacity">

      <rdfs:domain rdf:resource="#Device" />
      <rdfs:range rdf:resource="xsd:integer" />

      <rdfs:comment rdf:datatype="xsd:string">

         * This is a datatype property.

         A stock device has a fixed amount of disk capacity.

      </rdfs:comment>

   </owl:DatatypeProperty>

   <!-- ========================================= -->

   <owl:Class rdf:about="#Software">

      <owl:equivalentClass>
         <owl:Restriction>
            <owl:onProperty rdf:resource="#hasVersion" />
            <owl:cardinality rdf:datatype="xsd:nonNegativeInteger">1</owl:cardinality>
         </owl:Restriction>
      </owl:equivalentClass>

      <rdfs:comment rdf:datatype="xsd:string">

         * This is a cardinality restriction.

         Each piece of software can have at most 1 version. 
         Each version of software is considered to be a new instance. 
         Instance "Windows 7" is not the same as instance "Windows Vista".

      </rdfs:comment>

   </owl:Class>
   
   <!-- ========================================= -->
   
   <owl:FunctionalProperty rdf:about="#publishedBySource">
      
      <rdfs:domain rdf:resource="#News" />
      <rdfs:range rdf:resource="#NewsSource" />
      
      <rdfs:comment rdf:datatype="xsd:string">

         * This is a range restriction.

         Each piece of news can have only 1 source. 

      </rdfs:comment>
      
   </owl:FunctionalProperty>
   
   <!-- ========================================= -->
   
   <owl:InverseFunctionalProperty rdf:about="#sourcePublishedNews">
      
      <owl:inverseOf rdf:resource="#publishedBySource" />
      <rdfs:domain rdf:resource="#NewsSource" />
      <rdfs:range rdf:resource="#News" />
      
      <rdfs:comment rdf:datatype="xsd:string">

         * This is a domain restriction.
         * This is an inverse functional property.

         Each news source publishes some news. A single news
         item can only be published by 1 source. 

      </rdfs:comment>
      
   </owl:InverseFunctionalProperty>
   
   <!-- ========================================= -->
   
   <owl:ObjectProperty rdf:about="#withinRegion">
      
      <!-- 
         
         could use owl:TransitiveProperty but using the 
         alternative way to show that we know it 
         
      -->
      
      <rdf:type rdf:resource="&owl;TransitiveProperty" />
      <rdfs:domain rdf:resource="#Region" />
      <rdfs:range rdf:resource="#Region" />
      
      <rdfs:comment rdf:datatype="xsd:string">

         * This is a transitive property.
         * This is a (boring) domain restriction.
         * This is a (boring) range restriction.

         Each region can be contained within another region. 
         
            ~ Leicester is within England
            ~ England is within Global            
            ~ Leicester is within Global (implied)

      </rdfs:comment>
      
   </owl:ObjectProperty> 
   
   <!-- ========================================= -->
   
   <owl:TransitiveProperty rdf:about="#newerVersionThan">
      
      <rdfs:domain rdf:resource="#Device" />
      <rdfs:domain rdf:resource="#Software" />
      
      <rdfs:range rdf:resource="#Device" />
      <rdfs:range rdf:resource="#Software" />
      
      <rdfs:comment rdf:datatype="xsd:string">

         * This is a transitive property. 
         * This is a (boring) domain restriction.
         * This is a (boring) range restriction.
         
         An iPhone4S is a newerVersionThan iPhone3GS.         
         Windows 7 is a newerVersionThan Windows Vista.

      </rdfs:comment>
      
   </owl:ObjectProperty> 
   
   <!-- ========================================= -->
   
   <owl:Class rdf:about="#Device">
      
      <rdf:subClassOf>
         <owl:Restriction>
            <owl:onProperty rdf:resource="#newerVersionOf" />
            <owl:allValuesFrom rdf:resource="#Device" />
         </owl:Restriction>
      </rdf:subClassOf>
      
      <rdfs:comment rdf:datatype="xsd:string">

         * This is a universal restriction. 

         A device can only be a newer version of another device.

      </rdfs:comment>
      
   </owl:Class>
   
   <!-- ========================================= -->
   
   <owl:Class rdf:about="#Software">
      
      <rdfs:subClassOf>
         <owl:Restriction>
            <owl:onProperty rdf:resource="#newerVersionOf" />
            <owl:allValuesFrom rdf:resource="#Software" />
         </owl:Restriction>
      </rdfs:subClassOf>
      
      <rdfs:comment rdf:datatype="xsd:string">

         * This is a universal restriction. 

         A piece of software can only be a newer version of another piece of software.

      </rdfs:comment>
      
   </owl:Class>
   
   <!-- ========================================= -->

   <owl:Class rdf:about="#Newspaper">

      <owl:subClassOf>

         <owl:Restriction>
            <owl:onProperty rdf:resource="#hasCoverage" />
            <owl:minCardinality rdf:datatype="xsd:nonNegativeInteger">1</owl:minCardinality>
         </owl:Restriction>

         <rdfs:comment rdf:datatype="xsd:string">

            * This is a min cardinality restriction.

            A newspaper has coverage for at least 1 region. We include Global. 

         </rdfs:comment>

      </owl:subClassOf>

      <owl:subClassOf>

         <owl:Restriction>
            <owl:onProperty rdf:resource="#hasCorrespondingWebsite" />
            <owl:maxCardinality rdf:datatype="xsd:nonNegativeInteger">1</owl:maxCardinality>
         </owl:Restriction>
      
         <rdfs:comment rdf:datatype="xsd:string">

            * This is a max cardinality restriction.

            A newspaper has at most 1 corresponding website. 
   
         </rdfs:comment>

      </owl:subClassOf>

   </owl:Class>

   <!-- ========================================= -->

   <owl:SymmetricProperty rdf:about="#collaboratesWith">

      <rdfs:domain rdf:resource="#Journalist" />
      <rdfs:range rdf:resource="#Journalist" />

      <rdfs:comment rdf:datatype="xsd:string">

         * This is a symmetric property.

         Journalist 1 collaborates with Journalist 2.
         Journalist 2 collaborates with Journalist 1 (implied).

      </rdfs:comment>

   </owl:SymmetricProperty>

   <!-- ========================================= -->

   <owl:SymmetricProperty rdf:about="#canCommunicateWith">

      <rdfs:domain rdf:resource="#Device" />
      <rdfs:range rdf:resource="#Device" />

      <rdfs:comment rdf:datatype="xsd:string">

         * This is a symmetric property.

         An iPhone can communicate with a desktop computer (via network/usb). 
         A desktop computer can communicate with an iPhone (implied).

      </rdfs:comment>

   </owl:SymmetricProperty>

   <!-- ========================================= -->

   <owl:Class rdf:about="#Device">

      <owl:subClassOf>
         <owl:Restriction>
            <owl:onProperty rdf:resource="#runsSoftware" />
            <owl:someValuesFrom rdf:resource="#Software" />
         </owl:Restriction>
      </owl:subClassOf>

      <rdfs:comment rdf:datatype="xsd:string">

         * This is a existential restriction.

         Every device must run at least one piece of software. 
         Remember that firmware is considered software. 

      </rdfs:comment>
   
   </owl:Class>

   <!-- ========================================= -->
   
   <owl:InverseFunctionalProperty rdf:about="#hasPersonalBlog">
      
      <rdfs:domain rdf:resource="#Blogger" />
      <rdfs:range rdf:resource="#Blog" />
      
      <rdfs:comment rdf:datatype="xsd:string">

         * This is a domain restriction.
         * This is an inverse functional property.

         A blogger can have a personal blog. A single
         personal blog only belongs to exactly 1 person.

      </rdfs:comment>
      
   </owl:InverseFunctionalProperty>
      
   <!-- **************************************** -->
   <!--     INSTANCES OF NEW AND OLD CLASSES     -->
   <!-- **************************************** -->         
      
   <owl:NamedIndividual rdf:about="#Apple">
      <rdf:type rdf:resource="#Company"/>
   </owl:NamedIndividual>
      
</rdf:RDF>