<?xml version="1.0" encoding="utf-8" ?>

<!DOCTYPE rdf:RDF [
    <!ENTITY owl "http://www.w3.org/2002/07/owl#" >
    <!ENTITY xsd "http://www.w3.org/2001/XMLSchema#" >
    <!ENTITY rdfs "http://www.w3.org/2000/01/rdf-schema#" >
    <!ENTITY rdf "http://www.w3.org/1999/02/22-rdf-syntax-ns#" >
]>

<rdf:RDF 
   xmlns="http://docs.staite.net/uni-co7216-cwk2#"
   xml:base="http://docs.staite.net/uni-co7216-cwk2"
   xmlns:rdfs="http://www.w3.org/2000/01/rdf-schema#"
   xmlns:owl="http://www.w3.org/2002/07/owl#"
   xmlns:xsd="http://www.w3.org/2001/XMLSchema#"
   xmlns:rdf="http://www.w3.org/1999/02/22-rdf-syntax-ns#">
    
   <owl:Ontology rdf:about="http://docs.staite.net/uni-co7216-cwk2">
   
   
   </owl:Ontology>
   
   <!-- **************************************** -->   
   <!-- CLASSES AND PROPERTIES FROM COURSEWORK 1 -->  
   <!-- **************************************** -->
   
   <owl:Class rdf:about="#Region">
      <rdfs:comment rdf:datatype="xsd:string">
         [ Supporting Class ]
         Class of all geographical regions.
      </rdfs:comment>
   </owl:Class>   
   
   <owl:Class rdf:about="#News">
      <rdfs:comment rdf:datatype="xsd:string">
         [ Supporting Class ]
         Class of all news items.
      </rdfs:comment>
   </owl:Class>
   
   <owl:Class rdf:about="#NewsSubject">
      <rdfs:comment rdf:datatype="xsd:string">
         [ Supporting Class ]
         Class of all news subjects.
      </rdfs:comment>
   </owl:Class>   
   
   <owl:Class rdf:about="#NewsSource">
      <rdfs:comment rdf:datatype="xsd:string">
         [ Supporting Class ]
         Class of all news sources.
      </rdfs:comment>
   </owl:Class>
   
   <owl:Class rdf:about="#Person">
      <rdfs:comment rdf:datatype="xsd:string">
         [ Supporting Class ]
         Class of all people.
      </rdfs:comment>
   </owl:Class>

   <owl:Class rdf:about="#Journalist">
      <rdfs:subClassOf rdf:resource="#Person" />
      <rdfs:comment rdf:datatype="xsd:string">
         [ Supporting Class ]
         Class of all journalists.
      </rdfs:comment>
   </owl:Class>

   <owl:Class rdf:about="#Technology">
      <rdfs:subClassOf rdf:resource="#NewsSubject" />
      <rdfs:comment rdf:datatype="xsd:string">
         [ Supporting Class ]
         Class of all technology.
      </rdfs:comment>
   </owl:Class>

   <owl:Class rdf:about="#Software">
      <rdfs:subClassOf rdf:resource="#Technology" />
      <rdfs:comment rdf:datatype="xsd:string">
         [ Supporting Class ]
         Class of all software.
      </rdfs:comment>
   </owl:Class>

   <owl:Class rdf:about="#App">
      <rdfs:subClassOf rdf:resource="#Software" />
      <rdfs:comment rdf:datatype="xsd:string">
         [ Supporting Class ]
         Class of all applications.
      </rdfs:comment>
   </owl:Class>

   <owl:Class rdf:about="#OpenSource">
      <rdfs:subClassOf rdf:resource="#Technology" />
      <rdfs:comment rdf:datatype="xsd:string">
         [ Supporting Class ]
         Class of all open source technology.
      </rdfs:comment>
   </owl:Class>

   <owl:Class rdf:about="#Device">
      <rdfs:subClassOf rdf:resource="#Technology" />
      <rdfs:comment rdf:datatype="xsd:string">
         [ Supporting Class ]
         Class of all devices.
      </rdfs:comment>
   </owl:Class>

   <owl:Class rdf:about="#Mobile">
      <rdfs:subClassOf rdf:resource="#Device" />
      <rdfs:comment rdf:datatype="xsd:string">
         [ Supporting Class ]
         Class of all mobile devices.
      </rdfs:comment>
   </owl:Class>
   
   <owl:Class rdf:about="#Notebook">
     <rdfs:subClassOf rdf:resource="#Device" />
     <rdfs:comment rdf:datatype="xsd:string">
         [ Supporting Class ]
         Class of all notebook devices.
      </rdfs:comment>
   </owl:Class>
   
   <owl:Class rdf:about="#OS">
      <rdfs:subClassOf rdf:resource="#Software" />
      <rdfs:comment rdf:datatype="xsd:string">
         [ Supporting Class ]
         Class of all operating systems.
      </rdfs:comment>
   </owl:Class>

   <owl:Class rdf:about="#Company">
      <rdfs:subClassOf rdf:resource="#NewsSubject" />
      <rdfs:comment rdf:datatype="xsd:string">
         [ Supporting Class ]
         Class of all companies.
      </rdfs:comment>
   </owl:Class>

   <owl:Class rdf:about="#Newspaper">
      <rdfs:subClassOf rdf:resource="#NewsSource" />
      <rdfs:comment rdf:datatype="xsd:string">
         [ Supporting Class ]
         Class of all newspapers.
      </rdfs:comment>
   </owl:Class>
   
   <owl:Class rdf:about="#NewsWebsite">
      <rdfs:subClassOf rdf:resource="#NewsSource"/>
      <rdfs:comment rdf:datatype="xsd:string">
         [ Supporting Class ]
         Class of all news websites.
      </rdfs:comment>
   </owl:Class>
   
   <owl:Class rdf:about="#Desktop">
      <rdfs:subClassOf rdf:resource="#Device"/>
      <rdfs:comment rdf:datatype="xsd:string">
         [ Supporting Class ]
         Class of all desktop computers.
      </rdfs:comment>
   </owl:Class>
   
   <owl:Class rdf:about="#Independent">
      <rdfs:subClassOf rdf:resource="#NewsSource"/>
      <rdfs:comment rdf:datatype="xsd:string">
         [ Supporting Class ]
         Class of all independent news sources.
      </rdfs:comment>
   </owl:Class>
   
   <owl:Class rdf:about="#Blog">
      <rdfs:subClassOf rdf:resource="#Independent"/>
      <rdfs:comment rdf:datatype="xsd:string">
         [ Supporting Class ]
         Class of all blogs.
      </rdfs:comment>
   </owl:Class>
   
   <owl:Class rdf:about="#Developer">
      <rdfs:subClassOf rdf:resource="#NewsSubject"/>
      <rdfs:subClassOf rdf:resource="#Person"/>
      <rdfs:comment rdf:datatype="xsd:string">
         [ Supporting Class ]
         Class of all developers.
      </rdfs:comment>
   </owl:Class>
   
   <owl:ObjectProperty rdf:about="#runsSoftware">
      <rdfs:domain rdf:resource="#Device" />
      <rdfs:range rdf:resource="#Software" />
      <rdfs:comment rdf:datatype="xsd:string">
         [ Supporting Property ]
         A device runs software.
      </rdfs:comment>
   </owl:ObjectProperty>
   
   <owl:ObjectProperty rdf:about="#worksForSource">
      <rdfs:domain rdf:resource="#Journalist" />
      <rdfs:range rdf:resource="#NewsSource" />
      <rdfs:comment rdf:datatype="xsd:string">
         [ Supporting Property ]
         A journalist works for a news source.
      </rdfs:comment>
   </owl:ObjectProperty>

   <owl:ObjectProperty rdf:about="#builds">
      <rdfs:domain rdf:resource="#Company" />
      <rdfs:range rdf:resource="#Device" />
      <rdfs:comment rdf:datatype="xsd:string">
         [ Supporting Property ]
         A company builds a device.
      </rdfs:comment>
   </owl:ObjectProperty>

   <owl:ObjectProperty rdf:about="#hasCoverage">
      <rdfs:domain rdf:resource="#Newspaper" />
      <rdfs:range rdf:resource="#Region" />
      <rdfs:comment rdf:datatype="xsd:string">
         [ Supporting Property ]
         A newspaper has coverage in this/these regions.
      </rdfs:comment>
   </owl:ObjectProperty>    

   <owl:ObjectProperty rdf:about="#hasCorrespondingWebsite">
      <rdfs:range rdf:resource="#NewsWebsite"/>
      <rdfs:domain rdf:resource="#Newspaper"/>
      <rdfs:comment rdf:datatype="xsd:string">
         [ Supporting Property ]
         A newspaper has a corresponding website.
      </rdfs:comment>
   </owl:ObjectProperty>
   
   <owl:ObjectProperty rdf:about="#develops">
      <rdfs:domain>
         <owl:Class>
            <owl:unionOf rdf:parseType="Collection">
               <owl:Class rdf:about="#Developer" />
               <owl:Class rdf:about="#Company" />
            </owl:unionOf>
         </owl:Class>
      </rdfs:domain>
      <rdfs:range rdf:resource="#Software"/>
      <rdfs:comment rdf:datatype="xsd:string">
         [ Supporting Property ]
         A developer can develop software.
         A company can develop software.
      </rdfs:comment>
    </owl:ObjectProperty>

   <!-- **************************************** -->
   <!-- NEW CLASSES / PROPERTIES / RESTRICTIONS  -->
   <!-- **************************************** -->
   
   <owl:Class rdf:about="#Blogger">
   
      <rdfs:subClassOf rdf:resource="#Journalist" />
      <rdfs:subClassOf>
         <owl:Restriction>
            <owl:onProperty rdf:resource="#worksForSource" />
            <owl:someValuesFrom rdf:resource="#Blog" />
         </owl:Restriction>
      </rdfs:subClassOf>
      
      <rdfs:comment rdf:datatype="xsd:string">
      
         * This is a subclass restriction.
         * This is an existential restriction. 
         * This is an implicit cardinality restriction (min 1). 
         
         The class of people who are journalists and 
         work for at least 1 blog.         
      
      </rdfs:comment>
      
   </owl:Class>

   <!-- ========================================= -->

   <owl:ObjectProperty rdf:about="#runsOnDevice">

      <rdfs:domain rdf:resource="#Software" />
      <rdfs:range rdf:resource="#Device" />
      <owl:inverseOf rdf:resource="#runsSoftware" />

      <rdfs:comment rdf:datatype="xsd:string">
      
         * This is an object property.
         * This is an inverse property.
         * This is a (boring) domain restriction.
         * This is a (boring) range restriction.  
         
         A piece of software can run on 0 or more devices. 
      
      </rdfs:comment>

   </owl:ObjectProperty>

   <!-- ========================================= -->

   <owl:ObjectProperty rdf:about="#builtByCompany">

      <rdfs:domain rdf:resource="#Device" />
      <rdfs:range rdf:resource="#Company" />
      <owl:inverseOf rdf:resource="#builds" />

      <rdfs:comment rdf:datatype="xsd:string">
      
         * This is an object property.
         * This is an inverse property.
         * This is a (boring) domain restriction.
         * This is a (boring) range restriction.  
         
        A device is built by a company.
      
      </rdfs:comment>

   </owl:ObjectProperty>

   <!-- ========================================= -->

   <owl:Class rdf:about="#iPhoneDevice">
      
      <rdfs:subClassOf rdf:resource="#Mobile" />
      <rdfs:subClassOf>
         <owl:Restriction>
            <owl:onProperty rdf:resource="#builtByCompany" />
            <owl:hasValue rdf:resource="#Apple" />
         </owl:Restriction>
      </rdfs:subClassOf>

      <rdfs:comment>

         * This is a subclass restriction.
         * This is an (implicit) cardinality restriction (exactly 1).

         All mobile phones made by apple are iPhones. Note that
         the individuals are specific models like iPhone4S and
         iPhoneDevice is the class of these iPhone models. 

      </rdfs:comment>

   </owl:Class> 

   <!-- ========================================= -->

   <owl:Class rdf:about="#iPhoneApp">

      <rdfs:subClassOf rdf:resource="#App" />
      <rdfs:subClassOf>            
         <owl:Restriction>
            <owl:onProperty rdf:resource="#runsOnDevice" />
            <owl:allValuesFrom rdf:resource="#iPhoneDevice" />
         </owl:Restriction>
      </rdfs:subClassOf>

      <rdfs:comment rdf:datatype="xsd:string">

         * This is a subclass restriction.
         * This is a universal restriction. 

         Every iPhoneApp must be an App and it can only 
         run on an iPhoneDevice. 

      </rdfs:comment>

   </owl:Class>
      
   <!-- ========================================= -->

   <owl:Class rdf:about="#OpenSourceSoftware">

      <rdfs:subClassOf rdf:resource="#Software" />
      <rdfs:subClassOf rdf:resource="#OpenSource" />

      <rdfs:comment rdf:datatype="xsd:string">

         * This is a subclass restriction.

         The class of software that is open source. 

      </rdfs:comment>

   </owl:Class>

   <!-- ========================================= -->

   <owl:DatatypeProperty rdf:about="#hasVersion">

      <rdfs:domain rdf:resource="#Software" />
      <rdfs:range rdf:resource="&xsd;string" />

      <rdfs:comment rdf:datatype="xsd:string">

         * This is a datatype property.
         * This is a (boring) domain restriction.
         * This is a (boring) range restriction.  

         A piece of software has a version. 

      </rdfs:comment>

   </owl:DatatypeProperty>

   <!-- ========================================= -->

   <owl:DatatypeProperty rdf:about="#hasGBDiskCapacity">

      <rdfs:domain rdf:resource="#Device" />
      <rdfs:range rdf:resource="&xsd;nonNegativeInteger" />

      <rdfs:comment rdf:datatype="xsd:string">

         * This is a datatype property.

         A stock device has a fixed amount of disk capacity.

      </rdfs:comment>

   </owl:DatatypeProperty>

   <!-- ========================================= -->

   <owl:Class rdf:about="#Software">

      <owl:equivalentClass>
         <owl:Restriction>
            <owl:onProperty rdf:resource="#hasVersion" />
            <owl:cardinality rdf:datatype="xsd:nonNegativeInteger">1</owl:cardinality>
         </owl:Restriction>
      </owl:equivalentClass>

      <rdfs:comment rdf:datatype="xsd:string">

         * This is a cardinality restriction.

         Each piece of software can have at most 1 version. 
         Each version of software is considered to be a new instance. 
         Instance "Windows 7" is not the same as instance "Windows Vista".

      </rdfs:comment>

   </owl:Class>
   
   <!-- ========================================= -->
   
   <owl:FunctionalProperty rdf:about="#publishedBySource">
      
      <rdfs:domain rdf:resource="#News" />
      <rdfs:range rdf:resource="#NewsSource" />
      
      <rdfs:comment rdf:datatype="xsd:string">

         * This is a range restriction.

         Each piece of news can have only 1 source. 

      </rdfs:comment>
      
   </owl:FunctionalProperty>
   
   <!-- ========================================= -->
   
   <owl:InverseFunctionalProperty rdf:about="#sourcePublishedNews">
      
      <owl:inverseOf rdf:resource="#publishedBySource" />
      <rdfs:domain rdf:resource="#NewsSource" />
      <rdfs:range rdf:resource="#News" />
      
      <rdfs:comment rdf:datatype="xsd:string">

         * This is a domain restriction.
         * This is an inverse functional property.

         Each news source publishes some news. A single news
         item can only be published by 1 source. 

      </rdfs:comment>
      
   </owl:InverseFunctionalProperty>
   
   <!-- ========================================= -->
   
   <owl:ObjectProperty rdf:about="#withinRegion">
      
      <!-- 
         
         could use owl:TransitiveProperty but using the 
         alternative way to show that we know it 
         
      -->
      
      <rdf:type rdf:resource="&owl;TransitiveProperty" />
      <rdfs:domain rdf:resource="#Region" />
      <rdfs:range rdf:resource="#Region" />
      
      <rdfs:comment rdf:datatype="xsd:string">

         * This is a transitive property.
         * This is a (boring) domain restriction.
         * This is a (boring) range restriction.

         Each region can be contained within another region. 
         
            ~ Leicester is within England
            ~ England is within Global            
            ~ Leicester is within Global (implied)

      </rdfs:comment>
      
   </owl:ObjectProperty> 
   
   <!-- ========================================= -->
   
   <owl:TransitiveProperty rdf:about="#newerDeviceVersionThan">
      
      <rdfs:domain rdf:resource="#Device" />
      <rdfs:range rdf:resource="#Device" />
      
      <rdfs:comment rdf:datatype="xsd:string">

         * This is a transitive property. 
         * This is a (boring) domain restriction.
         * This is a (boring) range restriction.
         
         An iPhone4S is a newerDeviceVersionThan iPhone3GS.   

      </rdfs:comment>
      
   </owl:TransitiveProperty> 
   
   <!-- ========================================= -->
   
   <owl:TransitiveProperty rdf:about="#newerSoftwareVersionThan">
      
      <rdfs:domain rdf:resource="#Software" />
      <rdfs:range rdf:resource="#Software" />
      
      <rdfs:comment rdf:datatype="xsd:string">

         * This is a transitive property. 
         * This is a (boring) domain restriction.
         * This is a (boring) range restriction.
                 
         Windows 7 is a newerSoftwareVersionThan Windows Vista.

      </rdfs:comment>
      
   </owl:TransitiveProperty> 
   
   <!-- ========================================= -->
   
   <owl:Class rdf:about="#OpenSourceCompany">
      
      <rdfs:subClassOf>
         <owl:Restriction>
            <owl:onProperty rdf:resource="#develops" />
            <owl:allValuesFrom rdf:resource="#OpenSourceSoftware" />
         </owl:Restriction>
      </rdfs:subClassOf>
      
      <rdfs:subClassOf rdf:resource="#Company" />
      
      <rdfs:comment rdf:datatype="xsd:string">

         * This is a subclass restriction.
         * This is a universal restriction. 

         An open source company (Canonical) only develops open 
         source software (Ubuntu).

      </rdfs:comment>
      
   </owl:Class>
   
   <!-- ========================================= -->

   <owl:Class rdf:about="#Newspaper">

      <rdfs:subClassOf>
         <owl:Restriction>
            <owl:onProperty rdf:resource="#hasCoverage" />
            <owl:minCardinality rdf:datatype="xsd:nonNegativeInteger">1</owl:minCardinality>
            
            <rdfs:comment rdf:datatype="xsd:string">

               * This is a min cardinality restriction.

               A newspaper has coverage for at least 1 region. We include Global. 

            </rdfs:comment>
            
         </owl:Restriction>
      </rdfs:subClassOf>

      <rdfs:subClassOf>
         <owl:Restriction>
            
            <owl:onProperty rdf:resource="#hasCorrespondingWebsite" />
            <owl:maxCardinality rdf:datatype="xsd:nonNegativeInteger">1</owl:maxCardinality>
            
            <rdfs:comment rdf:datatype="xsd:string">

               * This is a max cardinality restriction.

               A newspaper has at most 1 corresponding website. 
      
            </rdfs:comment>
            
         </owl:Restriction>  
      </rdfs:subClassOf>

   </owl:Class>

   <!-- ========================================= -->

   <owl:SymmetricProperty rdf:about="#collaboratesWith">

      <rdfs:domain rdf:resource="#Journalist" />
      <rdfs:range rdf:resource="#Journalist" />

      <rdfs:comment rdf:datatype="xsd:string">

         * This is a symmetric property.

         Journalist 1 collaborates with Journalist 2.
         Journalist 2 collaborates with Journalist 1 (implied).

      </rdfs:comment>

   </owl:SymmetricProperty>

   <!-- ========================================= -->

   <owl:SymmetricProperty rdf:about="#canCommunicateWith">

      <rdfs:domain rdf:resource="#Device" />
      <rdfs:range rdf:resource="#Device" />

      <rdfs:comment rdf:datatype="xsd:string">

         * This is a symmetric property.

         An iPhone can communicate with a desktop computer (via network/usb). 
         A desktop computer can communicate with an iPhone (implied).

      </rdfs:comment>

   </owl:SymmetricProperty>

   <!-- ========================================= -->

   <owl:Class rdf:about="#Device">

      <rdfs:subClassOf>
         <owl:Restriction>
            <owl:onProperty rdf:resource="#runsSoftware" />
            <owl:someValuesFrom rdf:resource="#Software" />
         </owl:Restriction>
      </rdfs:subClassOf>

      <rdfs:comment rdf:datatype="xsd:string">

         * This is a existential restriction.

         Every device must run at least one piece of software. 
         Remember that firmware is considered software. 

      </rdfs:comment>
   
   </owl:Class>

   <!-- ========================================= -->
   
   <owl:InverseFunctionalProperty rdf:about="#hasPersonalBlog">
      
      <rdfs:domain rdf:resource="#Blogger" />
      <rdfs:range rdf:resource="#Blog" />
      
      <rdfs:comment rdf:datatype="xsd:string">

         * This is a domain restriction.
         * This is an inverse functional property.

         A blogger can have a personal blog. A single
         personal blog only belongs to exactly 1 person.

      </rdfs:comment>
      
   </owl:InverseFunctionalProperty>
      
   <!-- **************************************** -->
   <!--     INSTANCES OF NEW AND OLD CLASSES     -->
   <!-- **************************************** -->         
      
   <owl:NamedIndividual rdf:about="#Apple">
      <rdf:type rdf:resource="#Company"/>
      <rdfs:comment rdf:datatype="xsd:string">
         Apple is a Company.
         Apple builds iPhone 4S (implied).
      </rdfs:comment>
   </owl:NamedIndividual>
   
   <owl:NamedIndividual rdf:about="#JonathansBlog">
      <rdf:type rdf:resource="#Blog" />
      <rdfs:comment rdf:datatype="xsd:string">
         Jonathans Blog is a Blog.
         Jonathans Blog published the news item MyFirstBlogEntry (implied).
      </rdfs:comment>
   </owl:NamedIndividual>
   
   <owl:NamedIndividual rdf:about="#Jonathan">
      <rdf:type rdf:resource="#Blogger" />
      <collaboratesWith>
         <owl:NamedIndividual rdf:about="#Simone">
            <rdf:type rdf:resource="#Journalist" />
            <rdfs:comment rdf:datatype="xsd:string">
               Simone is a Journalist.
               Simone collaborates with Jonathan (implied).
            </rdfs:comment>
         </owl:NamedIndividual>
      </collaboratesWith>
      <hasPersonalBlog rdf:resource="#JonathansBlog" />
      <worksForSource rdf:resource="#LeicesterMercury" />
      <rdfs:comment rdf:datatype="xsd:string">
         Jonathan is a Blogger.
         Jonathan collaborates with Simone.
         Jonathan has the personal blog JonathansBlog.
         Jonathan works for the Leicester Mecury.
      </rdfs:comment>
   </owl:NamedIndividual>
   
   <owl:NamedIndividual rdf:about="#Ubuntu1110">
      <rdf:type rdf:resource="#OpenSourceSoftware" />
      <rdf:type rdf:resource="#OS" />
      <runsOnDevice>
         <owl:NamedIndividual rdf:about="#Dell_Inspiron_620">
            <rdf:type rdf:resource="#Desktop" />
            <builtByCompany>
               <!-- implies "builds" -->
               <owl:NamedIndividual rdf:about="#Dell">
                  <rdf:type rdf:resource="#Company" />
                  <rdfs:comment rdf:datatype="xsd:string">
                     Dell is a Company.
                     Dell builds the Inspiron 620 (implied).
                  </rdfs:comment>
               </owl:NamedIndividual>
            </builtByCompany>
            <hasGBDiskCapacity rdf:datatype="&xsd;nonNegativeInteger">500</hasGBDiskCapacity>
            <!-- implies "runsOnDevice" -->
            <runsSoftware rdf:resource="#Ubuntu1204" />
            <!-- implies "runsOnDevice" -->
            <runsSoftware rdf:resource="#Ubuntu1104" />
            <!-- implies "runsOnDevice" -->
            <runsSoftware rdf:resource="#Ubuntu1110" />
            <rdfs:comment rdf:datatype="xsd:string">
               Inspiron 620 is a desktop computer.
               Inspiron 620 is built by Dell.
               Inspiron 620 has 500GB hard disk. 
               Inspiron 620 runs Ubuntu 12.04.
               Inspiron 620 runs Ubuntu 11.04.
               Inspiron 620 runs Ubuntu 11.10.
               Inspiron 620 can communicate with iPhone 4S (implied).
            </rdfs:comment>
         </owl:NamedIndividual>
      </runsOnDevice>
      <hasVersion>11.10</hasVersion>      
      <newerSoftwareVersionThan rdf:resource="#Ubuntu1104" />
      <rdfs:comment rdf:datatype="xsd:string">
         Ubuntu 11.10 is an open source software.
         Ubuntu 11.10 is an OS.
         Ubuntu 11.10 runs on the Dell Inspiron 620.
         Ubuntu has version 11.10.
         Ubuntu 11.10 is newer than Ubuntu 11.04.
      </rdfs:comment>
   </owl:NamedIndividual>
   
   <owl:NamedIndividual rdf:about="#Ubuntu1204">
      <rdf:type rdf:resource="#OpenSourceSoftware" />
      <rdf:type rdf:resource="#OS" />
      <hasVersion>12.04</hasVersion>
      <newerSoftwareVersionThan rdf:resource="#Ubuntu1110" />
      <rdfs:comment rdf:datatype="xsd:string">
         Ubuntu 12.04 is an open source software.
         Ubuntu 12.04 is an OS.
         Ubuntu 12.04 runs on the Dell Inspiron 620 (implied).
         Ubuntu has version 12.04.
         Ubuntu 12.04 is newer than Ubuntu 11.10.
         Ubuntu 12.04 is newer than Ubuntu 11.04 (implied).
      </rdfs:comment>
   </owl:NamedIndividual>
   
   <!-- implies: Ubuntu1204 "newerSoftwareVersionThan" Ubuntu 1104 -->
   <owl:NamedIndividual rdf:about="#Ubuntu1104">
      <rdf:type rdf:resource="#OpenSourceSoftware" />
      <rdf:type rdf:resource="#OS" />
      <hasVersion>11.04</hasVersion>
      <rdfs:comment rdf:datatype="xsd:string">
         Ubuntu 11.04 is an open source software.
         Ubuntu 11.04 is an OS.
         Ubuntu 11.04 runs on the Dell Inspiron 620 (implied).
         Ubuntu has version 11.04.
      </rdfs:comment>
   </owl:NamedIndividual>
   
   <owl:NamedIndividual rdf:about="#Canonical">
      <rdf:type rdf:resource="#OpenSourceCompany" />
      <develops rdf:resource="#Ubuntu1104" />
      <develops rdf:resource="#Ubuntu1110" />
      <develops rdf:resource="#Ubuntu1204" />
      <rdfs:comment rdf:datatype="xsd:string">
         Canonical is an open source company. 
         Canonical develops Ubuntu 11.04, 11.10, 12.04. 
      </rdfs:comment>
   </owl:NamedIndividual>
   
   <owl:NamedIndividual rdf:about="#iPhone4S">
      <rdf:type rdf:resource="#iPhoneDevice" />
      <!-- implies: Dell Inspiron "canCommunicateWith" iPhone4S -->
      <canCommunicateWith rdf:resource="#Dell_Inspiron_620" />
      <runsSoftware rdf:resource="#MobileSafari" />
      <newerDeviceVersionThan>
         <owl:NamedIndividual rdf:about="iPhone4">
            <!-- implies: "builtByCompany" Apple -->
            <rdf:type rdf:resource="#iPhoneDevice" />
            <runsSoftware rdf:resource="#MobileSafari" />
            <rdfs:comment rdf:datatype="xsd:string">
               iPhone 4 is an iPhone Device.
               iPhone 4 is a Mobile (superclass of iPhoneDevice).
               iPhone 4 is built by Apple (implied).
               iPhone 4 runs Mobile Safari software.
            </rdfs:comment>
         </owl:NamedIndividual>
      </newerDeviceVersionThan>
      <rdfs:comment rdf:datatype="xsd:string">
         iPhone 4S is an iPhone Device.
         iPhone 4S is a Mobile (superclass of iPhoneDevice).
         iPhone 4S is built by Apple (implied).
         iPhone 4S can communicate with the Dell Inspiron 620.
         iPhone 4S runs Mobile Safari software.
         iPhone 4S is a new version of the iPhone 4.
      </rdfs:comment>
   </owl:NamedIndividual>
   
   <owl:NamedIndividual rdf:about="#MobileSafari">
      <rdf:type rdf:resource="#iPhoneApp" />
      <rdfs:comment rdf:datatype="xsd:string">
         Mobile Safari is an iPhone App.
         Mobile Safari runs only on iPhone devices (definition of iPhoneApp).
         Mobile Safari runs on iPhone 4S (implied).
         Mobile Safari runs on iPhone 4 (implied).
      </rdfs:comment>
   </owl:NamedIndividual>
   
   <owl:NamedIndividual rdf:about="#MyFirstBlogEntry">
      <rdf:type rdf:resource="#News" />
      <publishedBySource rdf:resource="#JonathansBlog" />
      <rdfs:comment rdf:datatype="xsd:string">
         MyFirstBlogEntry is a news item.
         MyFirstBlogEntry is published by Jonathans Blog.
      </rdfs:comment>
   </owl:NamedIndividual>
   
   <!-- implies: Leicester "withinRegion" Global -->
   <owl:NamedIndividual rdf:about="#Leicester">
      <rdf:type rdf:resource="#Region" />
      <withinRegion>
         <owl:NamedIndividual rdf:about="#England">
            <rdf:type rdf:resource="#Region" />
            <withinRegion>
               <owl:NamedIndividual rdf:about="#Global">
                  <rdf:type rdf:resource="#Region" />
                  <rdfs:comment rdf:datatype="xsd:string">
                     Global is a Region.
                  </rdfs:comment>
               </owl:NamedIndividual>
            </withinRegion>
            <rdfs:comment rdf:datatype="xsd:string">
               England is a Region.
               England is within Global.
            </rdfs:comment>
         </owl:NamedIndividual>
      </withinRegion>
      <rdfs:comment rdf:datatype="xsd:string">
         Leicester is a Region.
         Leicester is within England.
         Leicester is within Global (implied).
      </rdfs:comment>
   </owl:NamedIndividual>
   
   <owl:NamedIndividual rdf:about="#LeicesterMercury">
      <rdf:type rdf:resource="#Newspaper" />
      <hasCoverage rdf:resource="#Leicester" />
      <hasCorrespondingWebsite>
         <owl:NamedIndividual rdf:about="#ThisIsLeicestershireWebsite">
            <rdf:type rdf:resource="#NewsWebsite" />
            <rdfs:comment rdf:datatype="xsd:string">
               ThisIsLeicestershireWebsite is a news website.
            </rdfs:comment>
         </owl:NamedIndividual>
      </hasCorrespondingWebsite>
      <rdfs:comment rdf:datatype="xsd:string">
         Leicester Mercury is a newspaper.
         Leicester Mercury covers the region of Leicester.
         Leicester Mercury has corresponding website ThisIsLeicestershireWebsite.
      </rdfs:comment>
   </owl:NamedIndividual>
   
</rdf:RDF>